examples/ProcDecSC.v
@@ -1,0 +1,115 @@
+Require Import Bool String List.
+Require Import Lib.CommonTactics Lib.ilist Lib.Word Lib.Struct Lib.StringBound Lib.FMap.
+Require Import Lts.Syntax Lts.Semantics Lts.Inline Lts.Refinement.
+Require Import Ex.SC Ex.Fifo Ex.MemAtomic Ex.ProcDec.
+
+Require Import FunctionalExtensionality.
+
+Section ProcDecSC.
+  Variables addrSize fifoSize valSize rfIdx: nat.
+
+  Variable dec: DecT 2 addrSize valSize rfIdx.
+  Variable exec: ExecT 2 addrSize valSize rfIdx.
+
+  Definition procDecM (n: nat) := procDecM fifoSize dec exec n.
+  Definition sc (n: nat) := sc 2 _ _ _ dec exec opLd opSt opHt n.
+  Hint Unfold procDecM sc : ModuleDefs.
+
+  Section SingleCore.
+    Variable i: nat. (* i-th core *)
+    Notation "^ s" := (s __ i) (at level 0).
+
+    Definition pdecfi := ProcDec.pdecfi fifoSize dec exec i.
+    Definition pinsti := pinsti 2 _ _ _ dec exec opLd opSt opHt i.
+    Hint Unfold pdecfi pinsti.
+
+    Definition regRel: RegsT -> RegsT -> Prop.
+      intros ir sr.
+      refine (exists pcv: fullType type (SyntaxKind (Bit addrSize)),
+                M.find ^"pc" ir = Some {| objVal := pcv |} /\
+                _).
+      refine (exists rfv: fullType type (SyntaxKind (Vector (Bit valSize) rfIdx)),
+                M.find ^"rf" ir = Some {| objVal := rfv |} /\
+                _).
+      refine (exists eltsv: fullType type (SyntaxKind (Vector (atomK addrSize (Bit valSize))
+                                                              fifoSize)),
+                M.find (^"Outs" -n- "elt") ir = Some {| objVal := eltsv |} /\
+                _).
+      refine (exists deqPv: fullType type (SyntaxKind (Bit fifoSize)),
+                M.find (^"Outs" -n- "deqP") ir = Some {| objVal := deqPv |} /\
+                _).
+      refine (exists emptyv: fullType type (SyntaxKind Bool),
+                M.find (^"Outs" -n- "empty") ir = Some {| objVal := emptyv |} /\
+                _).
+      destruct emptyv.
+      - exact (sr = M.add ^"pc" {| objVal := pcv |}
+                                (M.add ^"rf" {| objVal := rfv |} (M.empty _))).
+      - pose (eltsv deqPv ``"type") as opcond.
+        destruct (weq opcond (evalConstT opLd)).
+        + refine (sr =
+                  M.add ^"pc" {| objVal := fst (exec _ rfv pcv (dec _ rfv pcv)) |}
+                              (M.add ^"rf" {| objType := SyntaxKind (Vector (Bit valSize) rfIdx);
+                                              objVal := _ |} (M.empty _))).
+          exact (fun a => if weq a (dec _ rfv pcv ``"reg")
+                          then eltsv deqPv ``"value"
+                          else rfv a).
+        + refine (sr =
+                  M.add ("pc"__ i) {| objVal := fst (exec _ rfv pcv (dec _ rfv pcv)) |}
+                        (M.add ("rf"__ i) {| objType := SyntaxKind (Vector (Bit valSize) rfIdx);
+                                             objVal := rfv |} (M.empty _))).
+    Defined.
+    Hint Unfold regRel.
+
+    Definition cmMap: CallsT -> CallsT := id.
+    Definition dmMap: CallsT -> CallsT := id.
+    Hint Unfold cmMap dmMap id.
+
+    Lemma Ht2t : t2t {dmMap, cmMap}.
+    Proof.
+      unfold t2t; intros.
+      destruct x as [[ ]]; simpl in *; subst; reflexivity.
+    Qed.
+
+    Definition ruleMap: string -> string :=
+      fun r =>
+        if string_eq r ("reqLd"__ i) then ("voidRule"__ i)
+        else if string_eq r ("reqSt"__ i) then ("voidRule"__ i)
+        else if string_eq r ("repLd"__ i) then ("voidRule"__ i)
+        else if string_eq r ("repSt"__ i) then ("voidRule"__ i)
+        else if string_eq r ("execHt"__ i) then ("execHt"__ i)
+        else if string_eq r ("execNm"__ i) then ("execNm"__ i)
+        else if string_eq r ("Mid"__ i -n- "processLd") then ("execLd"__ i)
+        else if string_eq r ("Mid"__ i -n- "processSt") then ("execSt"__ i)
+        else ("voidRule"__ i).
+    Hint Unfold ruleMap.
+
+    Definition f := f _ _ Ht2t.
+
+    Lemma procDec_SC_i: pdecfi <<=[f] pinsti.
+    Proof.
+      apply transMap with (regRel:=regRel) (ruleMap:=ruleMap).
+
+      - simpl; unfold regRel; repeat eexists;
+        try (repeat rewrite MF.find_add_2 by (intro; vdiscriminate);
+             rewrite MF.find_add_1; reflexivity); intuition auto.
+          
+      - admit.
+
+    Qed.
+
+  End SingleCore.
+
+  Theorem procDecM_SC: forall n, exists f, (procDecM n) <<=[f] (sc n).
+  Proof.
+    intros; exists id.
+    pose proof (procDec_SC_i).
+    unfold f, Refinement.f, dmMap, cmMap in H; rewrite <-id_idTrs in H by reflexivity.
+    repeat autounfold with ModuleDefs.
+
+    apply tr_comb.
+    - induction n; [apply H|]; simpl.
+      apply tr_comb; [apply H|assumption].
+    - apply tr_refl.
+  Qed.
+
+End ProcDecSC.
