src/SemanticsNew.v
@@ -1,7 +1,8 @@
 Require Import Lib.FMap Lib.Struct.
 Require Import Syntax Semantics Refinement.
-
 Require Import String List.
+
+Set Implicit Arguments.
 
 Record LabelTP {A : Type} :=
   { ruleMeth : option A
@@ -14,178 +15,166 @@ Arguments LabelTP : clear implicits.
 Definition LabelT := LabelTP True.
 Definition RuleLabelT := LabelTP string.
 
-Definition mapLabelTP {A B : Type} (f : A -> B) (l : LabelTP A) 
-  : LabelTP B := match l with
-  | Build_LabelTP rm dms cms => Build_LabelTP _ (option_map f rm) dms cms
+Definition mapLabelTP {A B : Type} (f : A -> B) (l : LabelTP A)
+: LabelTP B :=
+  match l with
+    | Build_LabelTP rm dms cms => Build_LabelTP (option_map f rm) dms cms
   end.
 
-Definition notBothRule (rm1 rm2 : option string) : Prop :=
+Definition NotBothRule (rm1 rm2 : option string) : Prop :=
   rm1 = None \/ rm2 = None.
 
 Inductive CanCombine : (RegsT * RuleLabelT) -> (RegsT * RuleLabelT) -> Prop :=
-  MkCanCombine : forall u1 rm1 ds1 cs1 u2 rm2 ds2 cs2,
-    MF.Disj u1 u2 -> MF.Disj ds1 ds2 -> MF.Disj cs1 cs2 
-  -> notBothRule rm1 rm2
-   -> CanCombine (u1, Build_LabelTP _ rm1 ds1 cs1) 
-                (u2, Build_LabelTP _ rm2 ds2 cs2).
+  MkCanCombine :
+    forall u1 rm1 ds1 cs1 u2 rm2 ds2 cs2,
+      MF.Disj u1 u2 -> MF.Disj ds1 ds2 -> MF.Disj cs1 cs2 
+      -> NotBothRule rm1 rm2
+      -> CanCombine (u1, Build_LabelTP rm1 ds1 cs1) 
+                    (u2, Build_LabelTP rm2 ds2 cs2).
 
-Definition mergeLabel {A : Type} (l1 l2 : LabelTP A) : LabelTP A 
- := match l1, l2 with
-  Build_LabelTP rm1 ds1 cs1, Build_LabelTP rm2 ds2 cs2 =>
-  Build_LabelTP _ 
-    (match rm1 with | Some r => Some r | None => rm2 end) 
-    (MF.union ds1 ds2) 
-    (MF.union cs1 cs2)
+Definition mergeLabel {A : Type} (l1 l2 : LabelTP A) : LabelTP A := 
+  match l1, l2 with
+      Build_LabelTP rm1 ds1 cs1, Build_LabelTP rm2 ds2 cs2 =>
+      Build_LabelTP (match rm1 with | Some r => Some r | None => rm2 end) 
+                    (MF.union ds1 ds2) 
+                    (MF.union cs1 cs2)
   end.
 
-Definition equivalent {A : Type} 
-  (l1 l2 : LabelTP A) (p : LabelTP A -> LabelTP A) :=
-   l1 = p l2.
+Definition equivalent {A : Type} (l1 l2 : LabelTP A)
+           (p : LabelTP A -> LabelTP A) :=
+  l1 = p l2.
 
 Local Open Scope string.
 
-Definition emptyStepName : string := "__empty__".
-
 Inductive UnitStep : Modules -> RegsT -> RegsT -> RuleLabelT -> Type :=
-| EmptyStep : forall
-   (regInits : list RegInitT)
-   (rules : list (Attribute (Action Void)))
-   (meths : list DefMethT)
-   (oRegs : RegsT)
-   (ruleMeth : bool),
-   MF.InDomain oRegs (namesOf regInits)
-   -> UnitStep (Mod regInits rules meths) oRegs (M.empty _)
-        (Build_LabelTP _ (if ruleMeth then Some emptyStepName else None)
-         (M.empty _) (M.empty _))
+| EmptyStep :
+    forall (regInits : list RegInitT)
+           (rules : list (Attribute (Action Void)))
+           (meths : list DefMethT)
+           (oRegs : RegsT),
+      MF.InDomain oRegs (namesOf regInits) ->
+      UnitStep (Mod regInits rules meths) oRegs (M.empty _)
+               (Build_LabelTP None (M.empty _) (M.empty _))
 | SingleRule : 
   forall (ruleName : string) (ruleBody : Action (Bit 0))
-   (regInits : list RegInitT)
-   (rules : list (Attribute (Action Void)))
-   (meths : list DefMethT)
-  , In (ruleName :: ruleBody)%struct rules ->
-  forall (oRegs news : RegsT) (calls : CallsT)
-  (retV : type (Bit 0)),
-  SemAction oRegs (ruleBody type) news calls retV ->
-   MF.InDomain oRegs (namesOf regInits) ->
-  UnitStep (Mod regInits rules meths) oRegs news
-       (Build_LabelTP _ (Some ruleName) (M.empty _) calls)
-| SingleMeth : forall 
-   (regInits : list RegInitT)
-   (rules : list (Attribute (Action Void)))
-   (meths : list DefMethT)
-   (oRegs : RegsT)
-   (calls : CallsT) (news : RegsT) 
-   (meth : DefMethT)
-   (argV : type (arg (objType (attrType meth))))
-   (retV : type (ret (objType (attrType meth))))
-   (udefs : CallsT),
-   SemAction oRegs (objVal (attrType meth) type argV) news calls retV ->
-   udefs = M.add meth {|
-                 objType := objType (attrType meth);
-                 objVal := (argV, retV) |} (M.empty _) ->
-   MF.InDomain oRegs (namesOf regInits) ->
-   UnitStep (Mod regInits rules meths) oRegs news
-      (Build_LabelTP _ None udefs calls)
-| LeftIntro : forall (m1 m2 : Modules)
-    (oRegs1 oRegs2 oRegs news : RegsT)
-    (l : RuleLabelT),
-    MF.InDomain oRegs2 (namesOf (getRegInits m2)) ->
-    UnitStep m1 oRegs1 news l ->
-    oRegs = MF.union oRegs1 oRegs2 ->
-    UnitStep (ConcatMod m1 m2) oRegs news l
-| RightIntro : forall (m1 m2 : Modules)
-    (oRegs1 oRegs2 oRegs news : RegsT)
-    (l : RuleLabelT),
-    MF.InDomain oRegs1 (namesOf (getRegInits m1)) ->
-    UnitStep m2 oRegs2 news l ->
-    oRegs = MF.union oRegs1 oRegs2 ->
-    UnitStep (ConcatMod m1 m2) oRegs news l.
+         (regInits : list RegInitT)
+         (rules : list (Attribute (Action Void)))
+         (meths : list DefMethT),
+    In (ruleName :: ruleBody)%struct rules ->
+    forall (oRegs news : RegsT) (calls : CallsT)
+           (retV : type (Bit 0)),
+      SemAction oRegs (ruleBody type) news calls retV ->
+      MF.InDomain oRegs (namesOf regInits) ->
+      UnitStep (Mod regInits rules meths) oRegs news
+               (Build_LabelTP (Some ruleName) (M.empty _) calls)
+| SingleMeth :
+    forall (regInits : list RegInitT)
+           (rules : list (Attribute (Action Void)))
+           (meths : list DefMethT)
+           (oRegs : RegsT)
+           (calls : CallsT) (news : RegsT) 
+           (meth : DefMethT)
+           (argV : type (arg (objType (attrType meth))))
+           (retV : type (ret (objType (attrType meth))))
+           (udefs : CallsT),
+      SemAction oRegs (objVal (attrType meth) type argV) news calls retV ->
+      udefs = M.add meth {|
+                      objType := objType (attrType meth);
+                      objVal := (argV, retV) |} (M.empty _) ->
+      MF.InDomain oRegs (namesOf regInits) ->
+      UnitStep (Mod regInits rules meths) oRegs news
+               (Build_LabelTP None udefs calls)
+| LeftIntro :
+    forall (m1 m2 : Modules)
+           (oRegs1 oRegs2 oRegs news : RegsT)
+           (l : RuleLabelT),
+      MF.InDomain oRegs2 (namesOf (getRegInits m2)) ->
+      UnitStep m1 oRegs1 news l ->
+      oRegs = MF.union oRegs1 oRegs2 ->
+      UnitStep (ConcatMod m1 m2) oRegs news l
+| RightIntro :
+    forall (m1 m2 : Modules)
+           (oRegs1 oRegs2 oRegs news : RegsT)
+           (l : RuleLabelT),
+      MF.InDomain oRegs1 (namesOf (getRegInits m1)) ->
+      UnitStep m2 oRegs2 news l ->
+      oRegs = MF.union oRegs1 oRegs2 ->
+      UnitStep (ConcatMod m1 m2) oRegs news l.
 
 Inductive UnitSteps (m : Modules) (o : RegsT) : RegsT -> RuleLabelT -> Type :=
- | UnitSteps1 : forall {u l}, UnitStep m o u l -> UnitSteps m o u l
- | UnitStepsUnion : forall {u1 u2 : RegsT} {l1 l2 : RuleLabelT}, 
-    UnitSteps m o u1 l1 -> UnitSteps m o u2 l2 
-    -> CanCombine (u1, l1) (u2, l2)
-    -> UnitSteps m o (MF.union u1 u2) (mergeLabel l1 l2).
+| UnitSteps1 : forall {u l}, UnitStep m o u l -> UnitSteps m o u l
+| UnitStepsUnion : forall {u1 u2 : RegsT} {l1 l2 : RuleLabelT}, 
+                     UnitSteps m o u1 l1 -> UnitSteps m o u2 l2 
+                     -> CanCombine (u1, l1) (u2, l2)
+                     -> UnitSteps m o (MF.union u1 u2) (mergeLabel l1 l2).
 
 Definition subtractKV {A : Type}
-  (deceqA : forall x y : A, sumbool (x = y) (x <> y))
-  (m1 m2 : M.t A) : M.t A :=
-    M.fold (fun k2 v2 m1' => match M.find k2 m1' with
-    | None => m1'
-    | Some v1 => if deceqA v1 v2 then 
-       M.remove k2 m1' else m1' 
-    end) m2 m1.
+           (deceqA : forall x y : A, sumbool (x = y) (x <> y))
+           (m1 m2 : M.t A) : M.t A :=
+  M.fold (fun k2 v2 m1' =>
+            match M.find k2 m1' with
+              | None => m1'
+              | Some v1 => if deceqA v1 v2 then 
+                             M.remove k2 m1' else m1' 
+            end) m2 m1.
 
-Definition signIsEq : forall (l1 l2 : Typed SignT),
-  sumbool (l1 = l2) (l1 <> l2).
-Proof. intros. destruct l1, l2. 
-destruct (SignatureT_dec objType objType0).
-- induction e. destruct objType, objVal, objVal0.
-  destruct (isEq arg t t1). induction e.
-  destruct (isEq ret t0 t2). induction e. left. reflexivity.
-  right. unfold not. intros. apply typed_eq in H.
-  inversion H. apply n in H1. assumption.
-  right. unfold not. intros. apply typed_eq in H.
-  inversion H. apply n in H1. assumption.
-- right. unfold not. intros. inversion H. apply n in H1.
-  assumption.
+Definition signIsEq :
+  forall (l1 l2 : Typed SignT), sumbool (l1 = l2) (l1 <> l2).
+Proof.
+  intros. destruct l1, l2. 
+  destruct (SignatureT_dec objType objType0).
+  - induction e. destruct objType, objVal, objVal0.
+    destruct (isEq arg t t1). induction e.
+    destruct (isEq ret t0 t2). induction e. left. reflexivity.
+    right. unfold not. intros. apply typed_eq in H.
+    inversion H. apply n in H1. assumption.
+    right. unfold not. intros. apply typed_eq in H.
+    inversion H. apply n in H1. assumption.
+  - right. unfold not. intros. inversion H. apply n in H1.
+    assumption.
 Qed.
 
-Definition hide {A : Type} (l : LabelTP A) : LabelTP A 
-  := match l with
-  Build_LabelTP rm ds cs => 
-    Build_LabelTP _ rm (subtractKV signIsEq ds cs)
-                       (subtractKV signIsEq cs ds)
+Definition hide {A : Type} (l : LabelTP A) : LabelTP A :=
+  match l with
+      Build_LabelTP rm ds cs => 
+      Build_LabelTP rm (subtractKV signIsEq ds cs)
+                    (subtractKV signIsEq cs ds)
   end.
 
-Definition wellHidden {A : Type} (l : LabelTP A) (m : Modules) 
-  := match l with
-    Build_LabelTP rm ds cs =>
-        MF.NotOnDomain ds (getCmsMod m)
+Definition wellHidden {A : Type} (l : LabelTP A) (m : Modules) :=
+  match l with
+      Build_LabelTP rm ds cs =>
+      MF.NotOnDomain ds (getCmsMod m)
       /\ MF.NotOnDomain cs (getDmsMod m)
   end.
 
 Inductive Step (m : Modules) (o u : RegsT) : RuleLabelT -> Type :=
-  MkStep : forall {l l': RuleLabelT}, UnitSteps m o u l
-   -> l' = hide l -> wellHidden l' m 
-   -> Step m o u l'.
+  MkStep : forall {l l': RuleLabelT},
+             UnitSteps m o u l ->
+             l' = hide l -> wellHidden l' m ->
+             Step m o u l'.
 
 Inductive MultiStep (m : Modules) (regs : RegsT) : RegsT -> list RuleLabelT -> Prop :=
 | MSNil : MultiStep m regs regs nil
-| MSMulti : forall regs' labels, MultiStep m regs regs' labels
-   -> forall l u, Step m regs' u l
-   -> forall (regs'' : RegsT), regs'' = update regs' u
-   -> MultiStep m regs regs'' (l :: labels).
+| MSMulti :
+    forall regs' labels,
+      MultiStep m regs regs' labels ->
+      forall l u,
+        Step m regs' u l ->
+        forall (regs'' : RegsT),
+          regs'' = update regs' u ->
+          MultiStep m regs regs'' (l :: labels).
 
 Inductive Behavior (m : Modules) : RegsT -> list LabelT -> Prop :=
- MkBehavior : forall newRegs labels labels'
-   , MultiStep m (initRegs (getRegInits m)) newRegs labels
-   -> labels' = (List.map (mapLabelTP (fun _ => I)) labels)
-   -> Behavior m newRegs labels'.
+  MkBehavior :
+    forall newRegs labels labels',
+      MultiStep m (initRegs (getRegInits m)) newRegs labels ->
+      labels' = (List.map (mapLabelTP (fun _ => I)) labels) ->
+      Behavior m newRegs labels'.
 
-Definition TraceRefines (mimpl mspec : Modules) (f : LabelT -> LabelT)
-  := forall simp limp,        Behavior mimpl simp         limp ->
-     exists (sspec : RegsT),  Behavior mspec sspec (map f limp).
-
-Set Implicit Arguments.
-
-Ltac destruct_match := 
-match goal with
-| [ |- context[ match ?e with | _ => _ end ]] => 
-   let x := fresh "eqn" in destruct e eqn:x
-end.
-
-Lemma union_disj_reorder {A : Type} : forall (m m1 m2 : M.t A),
-  MF.Disj m1 m2 -> MF.union m2 (MF.union m1 m)
-                = MF.union m1 (MF.union m2 m).
-Proof.
-intros. apply M.leibniz. unfold M.Equal. intros k.
-repeat rewrite MF.find_union.
-destruct (H k) as [H0 | H0];
-apply MF.F.P.F.not_find_in_iff in H0;
-repeat rewrite H0; destruct_match; reflexivity.
-Qed.
+Definition TraceRefines (mimpl mspec : Modules) (f : LabelT -> LabelT) :=
+  forall simp limp,        Behavior mimpl simp         limp ->
+  exists (sspec : RegsT),  Behavior mspec sspec (map f limp).
 
 Section Decomposition.
   Variable rulesImp rulesSpec: list string.
@@ -198,16 +187,16 @@ Section Decomposition.
   Definition pMod {A : Type} (f : A -> A) (l : LabelTP A) : LabelTP A
     := match l with
     | Build_LabelTP rm dm cm => let (dm', cm') := p (dm, cm) in
-       Build_LabelTP _ (option_map f rm) dm' cm'
+       Build_LabelTP (option_map f rm) dm' cm'
     end.
 
   Definition pRL := pMod ruleMap.
 
   Hypothesis pmerge : forall (ds1 ds2 cs1 cs2 : CallsT) (rm1 rm2 : option string)
-    , let l1 := Build_LabelTP _ rm1 ds1 cs1 in 
-      let l2 := Build_LabelTP _ rm2 ds2 cs2 in
+    , let l1 := Build_LabelTP rm1 ds1 cs1 in 
+      let l2 := Build_LabelTP rm2 ds2 cs2 in
        MF.Disj ds1 ds2 -> MF.Disj cs1 cs2
-     -> notBothRule rm1 rm2
+     -> NotBothRule rm1 rm2
      -> mergeLabel (pRL l1) (pRL l2) = pRL (mergeLabel l1 l2).
 
   Hypothesis phide : forall (l : RuleLabelT), pRL (hide l) = hide (pRL l).
@@ -279,7 +268,7 @@ Section Decomposition.
     destruct l2 as [rm2 ds2 cs2].
     inversion H; clear H; subst. 
     constructor; try (eapply MF.Disj_union_1; eassumption).
-    unfold notBothRule in *. destruct rm1; intuition.
+    unfold NotBothRule in *. destruct rm1; intuition.
   Qed.
 
   Lemma canCombineRight : forall {t u1 u2 l1 l2},
@@ -291,7 +280,7 @@ Section Decomposition.
     destruct l2 as [rm2 ds2 cs2].
     inversion H; clear H; subst. 
     constructor; try (eapply MF.Disj_union_2; eassumption).
-    unfold notBothRule in *. destruct rm1; intuition.
+    unfold NotBothRule in *. destruct rm1; intuition.
     congruence.
   Qed.
 
@@ -306,7 +295,7 @@ Section Decomposition.
     econstructor. apply MF.Disj_union; assumption.
     apply MF.Disj_union; assumption.
     apply MF.Disj_union; assumption.
-    unfold notBothRule in *; destruct rmL, rm2, rm4; intuition.
+    unfold NotBothRule in *; destruct rmL, rm2, rm4; intuition.
   Qed.  
 
   Lemma canCombineSym : forall {t1 t2},
@@ -315,7 +304,7 @@ Section Decomposition.
    intros t1 t2 H;
    inversion H; clear H; subst; 
    constructor; eauto using MF.Disj_comm.
-   unfold notBothRule in *.
+   unfold NotBothRule in *.
    destruct rm1, rm2; intuition.
   Qed. 
 
